Move operational semantics proofs to separate file

src/Prog.v
@@ -66,301 +66,32 @@ Inductive crash_step : forall T, prog T -> Prop :=
 | CrashWrite : forall a v,
     crash_step (Write a v).
 
-Module StepPresync.
-
-  Import Automation.
-
-  Hint Constructors step.
-  Hint Resolve possible_sync_trans.
-  Hint Resolve ListUtils.incl_cons2.
-
-  Theorem possible_sync_after_sync : forall A AEQ (m m': @mem A AEQ _),
-      possible_sync (sync_mem m) m' ->
-      m' = sync_mem m.
-  Proof.
-    unfold possible_sync, sync_mem; intros.
-    extensionality a.
-    specialize (H a).
-    destruct matches in *; intuition eauto;
-      repeat deex;
-      try congruence.
-    inversion H1; subst; eauto.
-    apply ListUtils.incl_in_nil in H3; subst; eauto.
-  Qed.
-
-  Lemma possible_sync_respects_upd : forall A AEQ (m m': @mem A AEQ _)
-                                       a v l l',
-      possible_sync m m' ->
-      incl l' l ->
-      possible_sync (upd m a (v, l)) (upd m' a (v,l')).
-  Proof.
-    unfold possible_sync; intros.
-    destruct (AEQ a a0); subst; autorewrite with upd;
-      intuition eauto.
-    specialize (H a0); intuition auto.
-    right; repeat eexists; eauto.
-    repeat deex.
-    right; repeat eexists; eauto.
-  Qed.
-
-  Hint Resolve incl_refl.
-
-  Lemma possible_sync_respects_sync_mem : forall A AEQ (m m': @mem A AEQ _),
-      possible_sync m m' ->
-      possible_sync (sync_mem m) (sync_mem m').
-  Proof.
-    unfold possible_sync, sync_mem; intros.
-    specialize (H a).
-    destruct matches; subst; intuition eauto;
-      try congruence;
-      repeat deex;
-      right;
-      cleanup.
-    do 3 eexists; intuition eauto.
-  Qed.
-
-  Hint Resolve possible_sync_respects_upd.
-  Hint Resolve possible_sync_respects_sync_mem.
-
-  Theorem step_presync : forall T (m m' m'' m''': rawdisk) hm (p: prog T) hm' v,
-      possible_sync (AEQ:=Nat.eq_dec) m m' ->
-      step m' hm p m'' hm' v ->
-      possible_sync (AEQ:=Nat.eq_dec) m'' m''' ->
-      exists (m'2: rawdisk),
-        step m hm p m'2 hm' v /\
-        possible_sync (AEQ:=Nat.eq_dec) m'2 m'''.
-  Proof.
-    intros.
-    inversion H0; subst; repeat sigT_eq; cleanup.
-    - exists m; intuition eauto.
-      specialize (H a); intuition auto; repeat deex; try congruence.
-      assert (v = v0) by congruence; subst.
-      eauto.
-    - pose proof (H a); intuition auto; try congruence.
-      repeat deex.
-      cleanup.
-      exists (upd m a (v0, v::l)).
-      intuition eauto.
-    - exists (sync_mem m).
-      intuition eauto.
-    - pose proof (H a); intuition auto; try congruence.
-      repeat deex.
-      cleanup.
-      exists (upd m a vs').
-      intuition eauto.
-      eapply possible_sync_trans; eauto.
-      destruct vs'.
-      eapply possible_sync_respects_upd; eauto.
-    - exists m; intuition eauto.
-  Qed.
-End StepPresync.
-
-Module ExecSync.
-
-  Inductive exec {sync_R: rawdisk -> rawdisk -> Prop} : forall T, rawdisk -> hashmap -> prog T -> outcome T -> Prop :=
-  | XRet : forall T m hm (v: T),
-      exec m hm (Ret v) (Finished m hm v)
-  | XStep : forall T m hm (p: prog T) m' m'' hm' v,
-      step m hm p m' hm' v ->
-      sync_R m' m'' ->
-      exec m hm p (Finished m'' hm' v)
-  | XBindFinish : forall m hm T (p1: prog T) m' hm' (v: T)
-                    T' (p2: T -> prog T') out,
-      exec m hm p1 (Finished m' hm' v) ->
-      exec m' hm' (p2 v) out ->
-      exec m hm (Bind p1 p2) out
-  | XBindFail : forall m hm T (p1: prog T)
-                  T' (p2: T -> prog T'),
-      exec m hm p1 (Failed T) ->
-      exec m hm (Bind p1 p2) (Failed T')
-  | XBindCrash : forall m hm T (p1: prog T) m' hm'
-                   T' (p2: T -> prog T'),
-      exec m hm p1 (Crashed T m' hm') ->
-      exec m hm (Bind p1 p2) (Crashed T' m' hm')
-  | XFail : forall m hm T (p: prog T),
-      fail_step m p ->
-      exec m hm p (Failed T)
-  | XCrash : forall m hm T (p: prog T),
-      crash_step p ->
-      exec m hm p (Crashed T m hm).
-
-  Arguments exec sync_R {T} _ _ _ _.
-
-End ExecSync.
-
-Require Import Automation.
-
-Arguments possible_sync {AT AEQ} _ _.
-
-Definition exec := @ExecSync.exec possible_sync.
-
-(* if out is ok, out' is at least as ok *)
-Definition outcome_obs_le T (out out': outcome T) : Prop :=
-  match out with
-  | Failed _ => out' = Failed T
-  | Finished d hm v => exists d', out' = Finished d' hm v /\
-                            possible_sync (AEQ:=addr_eq_dec) d d'
-  | Crashed _ d hm => exists d', out' = Crashed T d' hm /\
-                         possible_sync (AEQ:=addr_eq_dec) d d'
-  end.
-
-Definition outcome_obs_ge T (out' out: outcome T) : Prop :=
-  match out' with
-  | Failed _ => out = Failed T
-  | Finished d' hm v => exists d, out = Finished d hm v /\
-                             possible_sync (AEQ:=addr_eq_dec) d d'
-  | Crashed _ d' hm => exists d, out = Crashed T d hm /\
-                           possible_sync (AEQ:=addr_eq_dec) d d'
-  end.
-
-Theorem outcome_obs_ge_ok : forall T (out out': outcome T),
-    outcome_obs_le out out' <->
-    outcome_obs_ge out' out.
-Proof.
-  destruct out, out'; simpl; intuition idtac;
-    repeat deex;
-    match goal with
-    | [ H: @eq (outcome _) _ _ |- _ ] => inversion H; subst
-    end; eauto.
-Qed.
-
-Hint Resolve possible_sync_refl possible_sync_trans.
-
-Theorem outcome_obs_le_refl : forall T (out: outcome T),
-    outcome_obs_le out out.
-Proof.
-  destruct out; simpl; eauto.
-Qed.
-
-Theorem outcome_obs_le_trans : forall T (out out' out'': outcome T),
-    outcome_obs_le out out' ->
-    outcome_obs_le out' out'' ->
-    outcome_obs_le out out''.
-Proof.
-  destruct out, out'; intros; simpl in *; repeat deex; try congruence; eauto.
-  inversion H0; subst; eauto.
-  inversion H0; subst; eauto.
-Qed.
-
-Instance outcome_obs_le_preorder {T} : PreOrder (outcome_obs_le (T:=T)).
-Proof.
-  constructor; hnf; intros; eauto using outcome_obs_le_refl, outcome_obs_le_trans.
-Qed.
-
-Hint Constructors ExecSync.exec.
-
-Hint Resolve outcome_obs_le_refl outcome_obs_le_trans.
-
-Lemma possible_sync_in_domain : forall AT AEQ (d d': @mem AT AEQ _) a v vs',
-    possible_sync d d' ->
-    d' a = Some (v, vs') ->
-    exists vs, d a = Some (v, vs) /\
-          incl vs' vs.
-Proof.
-  unfold possible_sync; intros.
-  specialize (H a); intuition eauto; try congruence.
-  repeat deex.
-  assert (v = v0) by congruence; subst.
-  assert (l' = vs') by congruence; subst.
-  eauto.
-Qed.
-
-Lemma step_sync_later : forall T (p: prog T) d d' d'' hm hm' v,
-    possible_sync d d' ->
-    step d' hm p d'' hm' v ->
-    exists d'2, step d hm p d'2 hm' v /\
-           possible_sync (AEQ:=addr_eq_dec) d'2 d''.
-Proof.
-  intros.
-  inversion H0; subst; repeat sigT_eq.
-  - (* Read *)
-    eapply possible_sync_in_domain in H8; eauto; deex.
-    eauto.
-  - eapply possible_sync_in_domain in H8; eauto; deex.
-    eexists; split.
-    constructor; eauto.
-    eapply possible_sync_respects_upd; eauto.
-  - eauto.
-  - destruct vs, vs'.
-    eapply possible_sync_in_domain in H8; eauto; deex.
-    eexists; split.
-    econstructor; eauto.
-    eapply possible_sync_respects_upd; eauto.
-  - eauto.
-Qed.
-
-Lemma possible_sync_not_in_domain : forall AT AEQ (d d': @mem AT AEQ _) a,
-    possible_sync d d' ->
-    d' a = None ->
-    d a = None.
-Proof.
-  unfold possible_sync; intros.
-  specialize (H a); intuition eauto;
-    repeat deex; congruence.
-Qed.
-
-Hint Resolve possible_sync_not_in_domain.
-Hint Constructors fail_step.
-
-Lemma fail_step_sync_later  : forall T (p: prog T) d d',
-    fail_step d' p ->
-    possible_sync d d' ->
-    fail_step d p.
-Proof.
-  inversion 1; intros; subst; repeat sigT_eq; eauto.
-Qed.
-
-Theorem exec_eq_sync_later : forall T (p: prog T) d d' hm out,
-    ExecSync.exec eq d' hm p out ->
-    possible_sync d d' ->
-    exists out', ExecSync.exec eq d hm p out' /\
-            outcome_obs_ge out out'.
-Proof.
-  intros.
-  generalize dependent d.
-  induction H; subst; intros; simpl.
-  - eexists; intuition eauto; simpl; eauto.
-  - eapply step_sync_later in H0; eauto; deex.
-    eexists; intuition eauto.
-  - specialize (IHexec1 _ H1); deex.
-    simpl in *; deex.
-    specialize (IHexec2 _ H5); deex.
-    eauto 10.
-  - specialize (IHexec _ H0); deex.
-    simpl in *; subst.
-    eauto 10.
-  - specialize (IHexec _ H0); deex.
-    simpl in *; deex.
-    eauto 10.
-  - eapply fail_step_sync_later in H; eauto.
-  - inversion H; subst; repeat sigT_eq; eauto 10.
-Qed.
-
-Theorem exec_sync_obs_irrelevant : forall T (p: prog T) d hm out,
-    ExecSync.exec possible_sync d hm p out ->
-    exists out', ExecSync.exec eq d hm p out' /\
-            outcome_obs_le out' out.
-Proof.
-  induction 1; intros; repeat deex; eauto.
-  - eexists; intuition eauto.
-    simpl.
-    eauto.
-  - destruct out'0; simpl in *; repeat deex; try congruence.
-    inversion H5; subst.
-    (* m ---> m0, m0 ~~> d', d' ---> out' <= out *)
-    eapply exec_eq_sync_later in H4; eauto; deex.
-    simpl in *; deex.
-    assert (possible_sync (AEQ:=addr_eq_dec) d d') by eauto.
-    eapply exec_eq_sync_later in H1; eauto; deex.
-    apply outcome_obs_ge_ok in H9.
-    eauto.
-  - destruct out'; simpl in *; repeat deex; try congruence.
-    eauto.
-  - destruct out'; simpl in *; repeat deex; try congruence.
-    inversion H2; subst.
-    eexists; intuition eauto.
-    simpl; eauto.
-Qed.
+Inductive exec : forall T, rawdisk -> hashmap -> prog T -> outcome T -> Prop :=
+| XRet : forall T m hm (v: T),
+    exec m hm (Ret v) (Finished m hm v)
+| XStep : forall T m hm (p: prog T) m' m'' hm' v,
+    step m hm p m' hm' v ->
+    possible_sync m' m'' ->
+    exec m hm p (Finished m'' hm' v)
+| XBindFinish : forall m hm T (p1: prog T) m' hm' (v: T)
+                  T' (p2: T -> prog T') out,
+    exec m hm p1 (Finished m' hm' v) ->
+    exec m' hm' (p2 v) out ->
+    exec m hm (Bind p1 p2) out
+| XBindFail : forall m hm T (p1: prog T)
+                T' (p2: T -> prog T'),
+    exec m hm p1 (Failed T) ->
+    exec m hm (Bind p1 p2) (Failed T')
+| XBindCrash : forall m hm T (p1: prog T) m' hm'
+                 T' (p2: T -> prog T'),
+    exec m hm p1 (Crashed T m' hm') ->
+    exec m hm (Bind p1 p2) (Crashed T' m' hm')
+| XFail : forall m hm T (p: prog T),
+    fail_step m p ->
+    exec m hm p (Failed T)
+| XCrash : forall m hm T (p: prog T),
+    crash_step p ->
+    exec m hm p (Crashed T m hm).
 
 (** program with recovery *)
 Inductive recover_outcome (TF TR: Type) :=
@@ -368,80 +99,26 @@ Inductive recover_outcome (TF TR: Type) :=
   | RFinished (m: rawdisk) (hm: hashmap) (v: TF)
   | RRecovered (m: rawdisk) (hm: hashmap) (v: TR).
 
-Module ExecRecover.
-
-Inductive exec_recover {exec: forall T, rawdisk -> hashmap -> prog T -> outcome T -> Prop} (TF TR: Type)
+Inductive exec_recover (TF TR: Type)
     : rawdisk -> hashmap -> prog TF -> prog TR -> recover_outcome TF TR -> Prop :=
-  | XRFail : forall m hm p1 p2, exec _ m hm p1 (Failed TF)
+  | XRFail : forall m hm p1 p2, exec m hm p1 (Failed TF)
     -> exec_recover m hm p1 p2 (RFailed TF TR)
-  | XRFinished : forall m hm p1 p2 m' hm' (v: TF), exec _ m hm p1 (Finished m' hm' v)
+  | XRFinished : forall m hm p1 p2 m' hm' (v: TF), exec m hm p1 (Finished m' hm' v)
     -> exec_recover m hm p1 p2 (RFinished TR m' hm' v)
-  | XRCrashedFailed : forall m hm p1 p2 m' hm' m'r, exec _ m hm p1 (Crashed TF m' hm')
+  | XRCrashedFailed : forall m hm p1 p2 m' hm' m'r, exec m hm p1 (Crashed TF m' hm')
     -> possible_crash m' m'r
-    -> @exec_recover exec TR TR m'r hm' p2 p2 (RFailed TR TR)
+    -> @exec_recover TR TR m'r hm' p2 p2 (RFailed TR TR)
     -> exec_recover m hm p1 p2 (RFailed TF TR)
-  | XRCrashedFinished : forall m hm p1 p2 m' hm' m'r m'' hm'' (v: TR), exec _ m hm p1 (Crashed TF m' hm')
+  | XRCrashedFinished : forall m hm p1 p2 m' hm' m'r m'' hm'' (v: TR), exec m hm p1 (Crashed TF m' hm')
     -> possible_crash m' m'r
-    -> @exec_recover exec TR TR m'r hm' p2 p2 (RFinished TR m'' hm'' v)
+    -> @exec_recover TR TR m'r hm' p2 p2 (RFinished TR m'' hm'' v)
     -> exec_recover m hm p1 p2 (RRecovered TF m'' hm'' v)
-  | XRCrashedRecovered : forall m hm p1 p2 m' hm' m'r m'' hm'' (v: TR), exec _ m hm p1 (Crashed TF m' hm')
+  | XRCrashedRecovered : forall m hm p1 p2 m' hm' m'r m'' hm'' (v: TR), exec m hm p1 (Crashed TF m' hm')
     -> possible_crash m' m'r
-    -> @exec_recover exec TR TR m'r hm' p2 p2 (RRecovered TR m'' hm'' v)
+    -> @exec_recover TR TR m'r hm' p2 p2 (RRecovered TR m'' hm'' v)
     -> exec_recover m hm p1 p2 (RRecovered TF m'' hm'' v).
 
-Arguments exec_recover exec {TF TR} _ _ _ _ _.
-
-End ExecRecover.
-
-Definition exec_recover := @ExecRecover.exec_recover exec.
-
-Hint Constructors ExecRecover.exec_recover.
-
-Definition rout_obs_le TF TR (out out': recover_outcome TF TR) :=
- match out with
- | RFailed _ _ => out' = RFailed _ _
- | RFinished _ m hm v => exists m', out' = RFinished _ m' hm v /\
-                            possible_sync (AEQ:=addr_eq_dec) m m'
- | RRecovered _ m hm v => exists m', out' = RRecovered _ m' hm v /\
-                             possible_sync (AEQ:=addr_eq_dec) m m'
- end.
-
-Theorem exec_recover_obs_refinement : forall TF TR (p: prog TF) (r: prog TR)
-                                        d hm (P: recover_outcome TF TR -> Prop),
-    (forall d hm v d' hm' v', P (RFinished TR d hm v) ->
-                         outcome_obs_le (Finished d hm v) (Finished d' hm' v') ->
-                         P (RFinished TR d' hm' v')) ->
-    (forall out, ExecRecover.exec_recover (@ExecSync.exec eq) d hm p r out -> P out) ->
-    (forall out, ExecRecover.exec_recover (@ExecSync.exec possible_sync) d hm p r out -> P out).
-Proof.
-  intros.
-  induction H1; subst;
-  repeat match goal with
-         | [ H: ExecSync.exec possible_sync _ _ _ _ |- _ ] =>
-           apply exec_sync_obs_irrelevant in H; deex
-         | [ H: outcome_obs_le _ _ |- _ ] =>
-           apply outcome_obs_ge_ok in H; simpl in H
-         | _ => progress subst
-         | _ => deex
-         end.
-  - eauto.
-  - eapply H; eauto.
-    simpl; eauto.
-  - apply H0; eauto.
-    econstructor 3; eauto.
-    eapply possible_crash_possible_sync_trans; eauto.
-    admit. (* not clear if induction hypothesis can prove this *)
-  - apply H0; eauto.
-    econstructor 4; eauto.
-    eapply possible_crash_possible_sync_trans; eauto.
-    admit. (* similar induction hypothesis-based goal *)
-  - apply H0; eauto.
-    econstructor 5; eauto.
-    eapply possible_crash_possible_sync_trans; eauto.
-    admit. (* again same *)
-Abort.
-
-Hint Constructors GeneralExec.exec.
+Hint Constructors exec.
 Hint Constructors step.
 Hint Constructors exec_recover.
 
