src/OperationalSemantics.v
@@ -1,0 +1,309 @@
+Require Import Prog.
+Require Import AsyncDisk.
+Require Import Mem Pred PredCrash.
+Require Import Automation.
+
+Require Import FunctionalExtensionality.
+Require Import List.
+Require Import Arith.PeanoNat.
+Require Import RelationClasses.
+
+Set Implicit Arguments.
+
+Arguments possible_sync {AT AEQ} _ _.
+Hint Resolve possible_sync_refl.
+Hint Resolve possible_sync_trans.
+
+Section StepPreSync.
+Arguments possible_sync {AT AEQ} _ _.
+  Hint Constructors step.
+  Hint Resolve ListUtils.incl_cons2.
+
+  Theorem possible_sync_after_sync : forall A AEQ (m m': @mem A AEQ _),
+      possible_sync (sync_mem m) m' ->
+      m' = sync_mem m.
+  Proof.
+    unfold possible_sync, sync_mem; intros.
+    extensionality a.
+    specialize (H a).
+    destruct matches in *; intuition eauto;
+      repeat deex;
+      try congruence.
+    inversion H1; subst; eauto.
+    apply ListUtils.incl_in_nil in H3; subst; eauto.
+  Qed.
+
+  Lemma possible_sync_respects_upd : forall A AEQ (m m': @mem A AEQ _)
+                                       a v l l',
+      possible_sync m m' ->
+      incl l' l ->
+      possible_sync (upd m a (v, l)) (upd m' a (v,l')).
+  Proof.
+    unfold possible_sync; intros.
+    destruct (AEQ a a0); subst; autorewrite with upd;
+      intuition eauto.
+    specialize (H a0); intuition auto.
+    right; repeat eexists; eauto.
+    repeat deex.
+    right; repeat eexists; eauto.
+  Qed.
+
+  Hint Resolve incl_refl.
+
+  Lemma possible_sync_respects_sync_mem : forall A AEQ (m m': @mem A AEQ _),
+      possible_sync m m' ->
+      possible_sync (sync_mem m) (sync_mem m').
+  Proof.
+    unfold possible_sync, sync_mem; intros.
+    specialize (H a).
+    destruct matches; subst; intuition eauto;
+      try congruence;
+      repeat deex;
+      right;
+      cleanup.
+    do 3 eexists; intuition eauto.
+  Qed.
+
+  Hint Resolve possible_sync_respects_upd.
+  Hint Resolve possible_sync_respects_sync_mem.
+
+  Theorem step_presync : forall T (m m' m'' m''': rawdisk) hm (p: prog T) hm' v,
+      possible_sync (AEQ:=Nat.eq_dec) m m' ->
+      step m' hm p m'' hm' v ->
+      possible_sync (AEQ:=Nat.eq_dec) m'' m''' ->
+      exists (m'2: rawdisk),
+        step m hm p m'2 hm' v /\
+        possible_sync (AEQ:=Nat.eq_dec) m'2 m'''.
+  Proof.
+    intros.
+    inversion H0; subst; repeat sigT_eq; cleanup.
+    - exists m; intuition eauto.
+      specialize (H a); intuition auto; repeat deex; try congruence.
+      assert (v = v0) by congruence; subst.
+      eauto.
+    - pose proof (H a); intuition auto; try congruence.
+      repeat deex.
+      cleanup.
+      exists (upd m a (v0, v::l)).
+      intuition eauto.
+    - exists (sync_mem m).
+      intuition eauto.
+    - pose proof (H a); intuition auto; try congruence.
+      repeat deex.
+      cleanup.
+      exists (upd m a vs').
+      destruct vs'.
+      intuition eauto.
+    - exists m; intuition eauto.
+  Qed.
+End StepPreSync.
+
+Module Exec.
+
+  Inductive R {sync_R: rawdisk -> rawdisk -> Prop} : forall T, rawdisk -> hashmap -> prog T -> outcome T -> Prop :=
+  | XRet : forall T m hm (v: T),
+      R m hm (Ret v) (Finished m hm v)
+  | XStep : forall T m hm (p: prog T) m' m'' hm' v,
+      step m hm p m' hm' v ->
+      sync_R m' m'' ->
+      R m hm p (Finished m'' hm' v)
+  | XBindFinish : forall m hm T (p1: prog T) m' hm' (v: T)
+                    T' (p2: T -> prog T') out,
+      R m hm p1 (Finished m' hm' v) ->
+      R m' hm' (p2 v) out ->
+      R m hm (Bind p1 p2) out
+  | XBindFail : forall m hm T (p1: prog T)
+                  T' (p2: T -> prog T'),
+      R m hm p1 (Failed T) ->
+      R m hm (Bind p1 p2) (Failed T')
+  | XBindCrash : forall m hm T (p1: prog T) m' hm'
+                   T' (p2: T -> prog T'),
+      R m hm p1 (Crashed T m' hm') ->
+      R m hm (Bind p1 p2) (Crashed T' m' hm')
+  | XFail : forall m hm T (p: prog T),
+      fail_step m p ->
+      R m hm p (Failed T)
+  | XCrash : forall m hm T (p: prog T),
+      crash_step p ->
+      R m hm p (Crashed T m hm).
+
+  Arguments R sync_R {T} _ _ _ _.
+End Exec.
+
+Hint Constructors Exec.R.
+Hint Constructors exec.
+
+Theorem exec_is_exec_possible_sync : forall T (p: prog T) m hm out,
+    exec m hm p out <->
+    Exec.R possible_sync m hm p out.
+Proof.
+  split; induction 1; eauto.
+Qed.
+
+(* if out is ok, out' is at least as ok *)
+Definition outcome_obs_le T (out out': outcome T) : Prop :=
+  match out with
+  | Failed _ => out' = Failed T
+  | Finished d hm v => exists d', out' = Finished d' hm v /\
+                            possible_sync (AEQ:=addr_eq_dec) d d'
+  | Crashed _ d hm => exists d', out' = Crashed T d' hm /\
+                         possible_sync (AEQ:=addr_eq_dec) d d'
+  end.
+
+Definition outcome_obs_ge T (out' out: outcome T) : Prop :=
+  match out' with
+  | Failed _ => out = Failed T
+  | Finished d' hm v => exists d, out = Finished d hm v /\
+                             possible_sync (AEQ:=addr_eq_dec) d d'
+  | Crashed _ d' hm => exists d, out = Crashed T d hm /\
+                           possible_sync (AEQ:=addr_eq_dec) d d'
+  end.
+
+Theorem outcome_obs_ge_ok : forall T (out out': outcome T),
+    outcome_obs_le out out' <->
+    outcome_obs_ge out' out.
+Proof.
+  destruct out, out'; simpl; intuition idtac;
+    repeat deex;
+    match goal with
+    | [ H: @eq (outcome _) _ _ |- _ ] => inversion H; subst
+    end; eauto.
+Qed.
+
+Theorem outcome_obs_le_refl : forall T (out: outcome T),
+    outcome_obs_le out out.
+Proof.
+  destruct out; simpl; eauto.
+Qed.
+
+Theorem outcome_obs_le_trans : forall T (out out' out'': outcome T),
+    outcome_obs_le out out' ->
+    outcome_obs_le out' out'' ->
+    outcome_obs_le out out''.
+Proof.
+  destruct out, out'; intros; simpl in *; repeat deex; try congruence; eauto.
+  inversion H0; subst; eauto.
+  inversion H0; subst; eauto.
+Qed.
+
+Instance outcome_obs_le_preorder {T} : PreOrder (outcome_obs_le (T:=T)).
+Proof.
+  constructor; hnf; intros; eauto using outcome_obs_le_refl, outcome_obs_le_trans.
+Qed.
+
+Hint Resolve outcome_obs_le_refl outcome_obs_le_trans.
+
+Lemma possible_sync_in_domain : forall AT AEQ (d d': @mem AT AEQ _) a v vs',
+    possible_sync d d' ->
+    d' a = Some (v, vs') ->
+    exists vs, d a = Some (v, vs) /\
+          incl vs' vs.
+Proof.
+  unfold possible_sync; intros.
+  specialize (H a); intuition eauto; try congruence.
+  repeat deex.
+  assert (v = v0) by congruence; subst.
+  assert (l' = vs') by congruence; subst.
+  eauto.
+Qed.
+
+Hint Resolve ListUtils.incl_cons2.
+Hint Resolve incl_refl.
+Hint Resolve possible_sync_respects_sync_mem.
+
+Lemma step_sync_later : forall T (p: prog T) d d' d'' hm hm' v,
+    possible_sync d d' ->
+    step d' hm p d'' hm' v ->
+    exists d'2, step d hm p d'2 hm' v /\
+           possible_sync (AEQ:=addr_eq_dec) d'2 d''.
+Proof.
+  intros.
+  inversion H0; subst; repeat sigT_eq.
+  - (* Read *)
+    eapply possible_sync_in_domain in H8; eauto; deex.
+    eauto.
+  - eapply possible_sync_in_domain in H8; eauto; deex.
+    eexists; split.
+    constructor; eauto.
+    eapply possible_sync_respects_upd; eauto.
+  - eauto.
+  - destruct vs, vs'.
+    eapply possible_sync_in_domain in H8; eauto; deex.
+    eexists; split.
+    econstructor; eauto.
+    eapply possible_sync_respects_upd; eauto.
+  - eauto.
+Qed.
+
+Lemma possible_sync_not_in_domain : forall AT AEQ (d d': @mem AT AEQ _) a,
+    possible_sync d d' ->
+    d' a = None ->
+    d a = None.
+Proof.
+  unfold possible_sync; intros.
+  specialize (H a); intuition eauto;
+    repeat deex; congruence.
+Qed.
+
+Hint Resolve possible_sync_not_in_domain.
+Hint Constructors fail_step.
+
+Lemma fail_step_sync_later  : forall T (p: prog T) d d',
+    fail_step d' p ->
+    possible_sync d d' ->
+    fail_step d p.
+Proof.
+  inversion 1; intros; subst; repeat sigT_eq; eauto.
+Qed.
+
+Theorem exec_eq_sync_later : forall T (p: prog T) d d' hm out,
+    Exec.R eq d' hm p out ->
+    possible_sync d d' ->
+    exists out', Exec.R eq d hm p out' /\
+            outcome_obs_ge out out'.
+Proof.
+  intros.
+  generalize dependent d.
+  induction H; subst; intros; simpl.
+  - eexists; intuition eauto; simpl; eauto.
+  - eapply step_sync_later in H0; eauto; deex.
+    eexists; intuition eauto.
+  - specialize (IHR1 _ H1); deex.
+    simpl in *; deex.
+    specialize (IHR2 _ H5); deex.
+    eauto 10.
+  - specialize (IHR _ H0); deex.
+    simpl in *; subst.
+    eauto 10.
+  - specialize (IHR _ H0); deex.
+    simpl in *; deex.
+    eauto 10.
+  - eapply fail_step_sync_later in H; eauto.
+  - inversion H; subst; repeat sigT_eq; eauto 10.
+Qed.
+
+Theorem exec_sync_obs_irrelevant : forall T (p: prog T) d hm out,
+    Exec.R possible_sync d hm p out ->
+    exists out', Exec.R eq d hm p out' /\
+            outcome_obs_le out' out.
+Proof.
+  induction 1; intros; repeat deex; eauto.
+  - eexists; intuition eauto.
+    simpl.
+    eauto.
+  - destruct out'0; simpl in *; repeat deex; try congruence.
+    inversion H5; subst.
+    (* m ---> m0, m0 ~~> d', d' ---> out' <= out *)
+    eapply exec_eq_sync_later in H4; eauto; deex.
+    simpl in *; deex.
+    assert (possible_sync (AEQ:=addr_eq_dec) d d') by eauto.
+    eapply exec_eq_sync_later in H1; eauto; deex.
+    apply outcome_obs_ge_ok in H9.
+    eauto.
+  - destruct out'; simpl in *; repeat deex; try congruence.
+    eauto.
+  - destruct out'; simpl in *; repeat deex; try congruence.
+    inversion H2; subst.
+    eexists; intuition eauto.
+    simpl; eauto.
+Qed.
